%% AMS-LaTeX Created by Wolfram Mathematica 9.0 : www.wolfram.com

\documentclass{article}
\usepackage{amsmath, amssymb, graphics, setspace}

\newcommand{\mathsym}[1]{{}}
\newcommand{\unicode}[1]{{}}

\begin{document}

\begin{doublespace}
\noindent\(\pmb{C_{(p,N)}+C_{(p,N-1)}=C_{(p+1,N)}}\\
\pmb{\underset{k=0}{\overset{N-1}{2\sum }}\left(
\begin{array}{c}
 p-1 \\
 k \\
\end{array}
\right) + \underset{k=0}{\overset{N-1-1}{2\sum }}\left(
\begin{array}{c}
 p-1 \\
 k \\
\end{array}
\right) = \underset{k=0}{\overset{N-1}{2\sum }}\left(
\begin{array}{c}
 p \\
 k \\
\end{array}
\right)}\\
\pmb{\sum _{k=0}^{N-1} \left(
\begin{array}{c}
 p-1 \\
 k \\
\end{array}
\right) + \sum _{k=0}^{N-2} \left(
\begin{array}{c}
 p-1 \\
 k \\
\end{array}
\right) = \sum _{k=0}^{N-1} \left(
\begin{array}{c}
 p \\
 k \\
\end{array}
\right)}\\
\pmb{1+\sum _{k=1}^{N-1} \left(
\begin{array}{c}
 p-1 \\
 k \\
\end{array}
\right) + \sum _{k=0}^{N-2} \left(
\begin{array}{c}
 p-1 \\
 k \\
\end{array}
\right) =1+ \sum _{k=1}^{N-1} \left(
\begin{array}{c}
 p \\
 k \\
\end{array}
\right)}\\
\pmb{\sum _{k=1}^{N-1} \left(
\begin{array}{c}
 p-1 \\
 k \\
\end{array}
\right) + \sum _{k=0}^{N-2} \left(
\begin{array}{c}
 p-1 \\
 k \\
\end{array}
\right) =\sum _{k=1}^{N-1} \left(
\begin{array}{c}
 p \\
 k \\
\end{array}
\right)}\\
\pmb{\sum _{k=1}^{N-1} \left(
\begin{array}{c}
 p-1 \\
 k \\
\end{array}
\right) + \sum _{k=1}^{N-1} \left(
\begin{array}{c}
 p-1 \\
 k-1 \\
\end{array}
\right) =\sum _{k=1}^{N-1} \left(
\begin{array}{c}
 p \\
 k \\
\end{array}
\right)}\\
\pmb{\sum _{k=1}^{N-1} \left(\left(
\begin{array}{c}
 p-1 \\
 k \\
\end{array}
\right)+\left(
\begin{array}{c}
 p-1 \\
 k-1 \\
\end{array}
\right)\right) =\sum _{k=1}^{N-1} \left(
\begin{array}{c}
 p \\
 k \\
\end{array}
\right)}\\
\pmb{\left(
\begin{array}{c}
 p-1 \\
 k \\
\end{array}
\right)+\left(
\begin{array}{c}
 p-1 \\
 k-1 \\
\end{array}
\right) =\left(
\begin{array}{c}
 p \\
 k \\
\end{array}
\right)}\)
\end{doublespace}

\end{document}
